new/proof/github_com/goose_lang/goose/testdata/examples/lock.v
@@ -5,32 +5,32 @@ From New.proof.github_com.goose_lang.goose.model.channel Require Import
   idiom.base lock bag.
 From New.proof Require Import github_com.goose_lang.goose.model.channel.idiom.closeable.closeable.
 From New.proof Require Import time.
-From New.generatedproof.github_com.goose_lang.goose.testdata.examples Require Import channel.
-Import New.code.github_com.goose_lang.goose.testdata.examples.channel.chan_spec_raw_examples.
+From New.generatedproof.github_com.goose_lang.goose.testdata.examples.channel Require Import lock.
+Import New.code.github_com.goose_lang.goose.testdata.examples.channel.lock.lock.
 
 Set Default Proof Using "Type".
 
 Section proof.
 Context `{hG: heapGS Σ, !ffi_semantics _ _}.
-Context {sem : go.Semantics} {package_sem : chan_spec_raw_examples.Assumptions}.
+Context {sem : go.Semantics} {package_sem : lock.Assumptions}.
 
-#[global] Instance : IsPkgInit (iProp Σ) chan_spec_raw_examples := define_is_pkg_init True%I.
-#[global] Instance : GetIsPkgInitWf (iProp Σ) chan_spec_raw_examples := build_get_is_pkg_init_wf.
+#[global] Instance : IsPkgInit (iProp Σ) pkg_id.lock := define_is_pkg_init True%I.
+#[global] Instance : GetIsPkgInitWf (iProp Σ) pkg_id.lock := build_get_is_pkg_init_wf.
 Collection W := sem + package_sem.
 Set Default Proof Using "W".
 
-Definition is_Lock (γ : lock_channel_names) (l : chan_spec_raw_examples.Lock.t) (R : iProp Σ) : iProp Σ :=
+Definition is_Lock (γ : lock_channel_names) (l : lock.Lock.t) (R : iProp Σ) : iProp Σ :=
   "#Hlock_chan" ∷ is_lock_channel (V:=unit) γ (Lock.ch' l) R.
 
 #[global] Instance is_Lock_persistent γ l R : Persistent (is_Lock γ l R) := _.
 
 
 Lemma wp_NewLock (R : iProp Σ) :
-  {{{ is_pkg_init chan_spec_raw_examples ∗ ▷ R }}}
-    @! chan_spec_raw_examples.NewLock #()
+  {{{ is_pkg_init pkg_id.lock ∗ ▷ R }}}
+    @! lock.NewLock #()
   {{{ γ l, RET #l; is_Lock γ l R }}}.
   Proof using ext ffi ffi_interp0 ffi_semantics0 hG package_sem sem Σ.
-  wp_start as "HR". 
+  wp_start as "HR".
   wp_apply chan.wp_make2; first done.
   iIntros (ch γch) "(#Hchan & %Hcap & Hoc)".
   rewrite -wp_fupd.
@@ -44,12 +44,12 @@ Lemma wp_NewLock (R : iProp Σ) :
 Qed.
 
 Lemma wp_Lock__Lock γ l (R : iProp Σ) :
-  {{{ is_pkg_init chan_spec_raw_examples ∗ is_Lock γ l R }}}
-   l @! chan_spec_raw_examples.Lock @! "Lock" #()
+  {{{ is_pkg_init pkg_id.lock ∗ is_Lock γ l R }}}
+   l @! lock.Lock @! "Lock" #()
   {{{ RET #(); R }}}.
 Proof.
   wp_start.
-  iNamed "Hpre". 
+  iNamed "Hpre".
   wp_auto.
   wp_apply ((wp_lock_channel_lock (t:=(go.StructType [])) γ l.(Lock.ch') ) with "[$Hchan //]").
   iIntros "HR".
@@ -58,13 +58,13 @@ Proof.
 Qed.
 
 Lemma wp_Lock__Unlock γ l (R : iProp Σ) :
-  {{{ is_pkg_init chan_spec_raw_examples ∗
+  {{{ is_pkg_init pkg_id.lock ∗
       is_Lock γ l R ∗ R }}}
-   l @! chan_spec_raw_examples.Lock @! "Unlock" #()
+   l @! lock.Lock @! "Unlock" #()
   {{{ RET #(); True }}}.
 Proof.
   wp_start.
-  iNamed "Hpre". 
+  iNamed "Hpre".
   iDestruct "Hpre" as "(#Hheld & HR)".
   wp_auto.
   iNamed "Hheld".
@@ -74,8 +74,8 @@ Proof.
 Qed.
 
 Lemma wp_Lock__TryLock γ (l : Lock.t) (R : iProp Σ) :
-  {{{ is_pkg_init chan_spec_raw_examples ∗ is_Lock γ l R }}}
-   l @! chan_spec_raw_examples.Lock @! "TryLock" #()
+  {{{ is_pkg_init pkg_id.lock ∗ is_Lock γ l R }}}
+   l @! lock.Lock @! "TryLock" #()
   {{{ (b : bool), RET #b; if b then R else True }}}.
 Proof.
   wp_start.
@@ -95,10 +95,10 @@ Qed.
 Lemma wp_Lock__LockIfNotCancelled
     γlock (l: Lock.t) (done_ch : chan.t) (R Q : iProp Σ)
     (γdone : chan_names) `{!Persistent Q}:
-  {{{ is_pkg_init chan_spec_raw_examples ∗
+  {{{ is_pkg_init pkg_id.lock ∗
       is_Lock γlock l R ∗
       own_closeable_chan done_ch γdone Q closeable.Unknown }}}
-   l @! chan_spec_raw_examples.Lock @! "LockIfNotCancelled" #done_ch
+   l @! lock.Lock @! "LockIfNotCancelled" #done_ch
   {{{ (b : bool), RET #b;
       if b then R else Q }}}.
 Proof.
@@ -124,8 +124,8 @@ Proof.
 Qed.
 
 Lemma wp_Lock__LockWithTimeout γ (l : Lock.t) (R : iProp Σ) (d : time.Duration.t) :
-  {{{ is_pkg_init chan_spec_raw_examples ∗ is_Lock γ l R }}}
-   l @! chan_spec_raw_examples.Lock @! "LockWithTimeout" #d
+  {{{ is_pkg_init pkg_id.lock ∗ is_Lock γ l R }}}
+   l @! lock.Lock @! "LockWithTimeout" #d
   {{{ (b : bool), RET #b;
       if b then R else True }}}.
 Proof.
@@ -137,7 +137,7 @@ Proof.
   wp_bind.
   wp_apply (wp_After).
   iIntros (after_ch γafter_ch) "#Hafter_chan".
-  wp_auto_lc 2. 
+  wp_auto_lc 2.
   wp_apply chan.wp_select_blocking. simpl.
    iSplit.
   - simpl. iExists unit, l.(Lock.ch'), γ.(lchan_name), tt, _, _, _.
@@ -147,9 +147,9 @@ Proof.
     wp_auto. iApply "HΦ". iFrame.
   - iSplitL; last done.
     simpl. iExists time.Time.t, after_ch.
-    iFrame "#". iFrame. 
+    iFrame "#". iFrame.
      repeat iExists _.
-    iSplitR; first done. 
+    iSplitR; first done.
     iDestruct (is_bag_is_chan with "Hafter_chan") as "#H".
     iFrame "#".
     iApply (bag_recv_au with "[$] [$Hafter_chan]").
